coq/SystemFTest.v
@@ -25,89 +25,6 @@ Import ListNotations.
 Import MonadNotation.
 Local Open Scope monad_scope.
 
-Variant Precedence :=
-| PrecOuter
-| PrecMult
-| PrecAdd
-| PrecSub
-| PrecApp
-| PrecInner
-.
-
-Definition prec_value (p : Precedence) : N :=
-  match p with
-  | PrecOuter => 0
-  | PrecAdd => 1
-  | PrecSub => 1
-  | PrecMult => 2
-  | PrecApp => 3
-  | PrecInner => 4
-  end.
-
-Definition parens (outer inner : Precedence) (s : string) :=
-  if N.leb (prec_value outer) (prec_value inner)
-  then s
-  else "(" ++ s ++ ")".
-
-Definition intersperse (sep : string) (l : list string) : string
-  := fold_left (fun acc s => if eqb "" acc then s else s ++ sep ++ acc) l "".
-
-Fixpoint showFType_helper (prec : Precedence) (t : FType) :=
-  match t with
-  | Arrow a b => parens prec PrecApp (showFType_helper PrecInner a ++ "->" ++ showFType_helper PrecApp b)
-  | Prod ts => "<" ++ intersperse ", " (map (showFType_helper PrecOuter) ts) ++ ">"
-  | TForall t => parens prec PrecOuter ("forall " ++ showFType_helper PrecOuter t)
-  | TVar x => "t" ++ show x
-  | IntType => "Int"
-  end.
-
-Instance showFType : Show FType := 
-  {| show := showFType_helper PrecOuter
-  |}.
-
-Instance showPrimOp : Show PrimOp :=
-  {| show :=
-       fun (op : PrimOp) =>
-         match op with
-         | Mul => "*"
-         | Add => "+"
-         | Sub => "-"
-         end
-  |}.
-
-Definition op_prec (op : PrimOp) : Precedence
-  := match op with
-     | Mul => PrecMult
-     | Add => PrecAdd
-     | Sub => PrecSub
-     end.           
-
-Fixpoint showTerm_helper {I} `{FInt I} `{Show I} (prec : Precedence) (e : Term) :=
-  match e with
-  | Var x => "v" ++ show x
-  | Ann e t => parens prec PrecOuter (showTerm_helper PrecOuter e ++ " : " ++ show t)
-  | Fix ft t body => parens prec PrecOuter ("λ " ++ show ft ++ " " ++ show t ++ ". " ++ showTerm_helper PrecOuter body)
-  | TAbs e => parens prec PrecOuter ("Λ. " ++ showTerm_helper PrecOuter e)
-  | App e1 e2 => parens prec PrecInner (showTerm_helper PrecInner e1 ++ " " ++ showTerm_helper PrecApp e2)
-  | TApp e t => parens prec PrecInner (showTerm_helper PrecInner e ++ " [" ++ show t ++ "]")
-  | Tuple es => "<" ++ intersperse ", " (map (showTerm_helper PrecOuter) es) ++ ">"
-  | ProjN i e => parens prec PrecInner ("π" ++ show i ++ " " ++ showTerm_helper PrecApp e)
-  | Num n => show n
-  | If0 c e1 e2 => parens prec PrecApp ("if0 " ++ showTerm_helper PrecOuter c ++ " then " ++ showTerm_helper PrecOuter e1 ++ " else " ++ showTerm_helper PrecOuter e2)
-  | Op op e1 e2 =>
-    let oprec := op_prec op in
-    parens prec oprec (showTerm_helper oprec e1 ++ " " ++ show op ++ " " ++ showTerm_helper oprec e2) 
-  end.
-
-Instance showInt64 : Show Int64.int :=
-  {| show := fun i => show (Int64.intval i)
-  |}.
-
-Instance showTerm {I} `{FInt I} `{Show I} : Show Term :=
-  {| show := showTerm_helper PrecOuter
-  |}.
-
-
 Definition elems_fail {A : Type} (l : list A) :=
   let n := length l in
   bindGen (choose (0, n - 1))
@@ -597,9 +514,8 @@ Instance showMLResult {A E} `{Show A} `{Show E} : Show (MlResult A E)
             end
     |}.
 
-
 (* Test that we evaluate without failing *)
-QuickCheck (forAll (genFType 0) (fun τ => forAll (genTerm_terminating 0 [] τ)
+QuickCheck (forAll (genFType 0) (fun τ => forAllShrink (genTerm_terminating 0 [] τ) shrink_term_preserve_type
                                               (fun e => match run_eval (eval e) with
                                                      | MlOk _ =>
                                                        checker true
